Pushing the main result.

concurrency/HybridMachine_simulation.v
@@ -1,4 +1,5 @@
 From mathcomp.ssreflect Require Import ssreflect seq ssrbool ssrfun.
+Require Import Coqlib.
 Require Import compcert.common.Memory.
 Require Import compcert.common.AST.     (*for typ*)
 Require Import compcert.common.Values. (*for val*)
@@ -45,52 +46,39 @@ Require Import compcert.common.Smallstep.
 Require Import concurrency.machine_semantics_lemmas.
 
 
+Set Bullet Behavior "Strict Subproofs".
+
 Section HybridSimulation.
 
   Variable (Sems Semt : Semantics_rec).
   Variable (hb1 hb2: option nat).
 
-  Definition Resources : Resources_rec:=
-    Build_Resources_rec (access_map * access_map)%type (access_map * access_map)%type.
-  
-  Definition HM1:=HybridMachine hb1 Sems Semt.
-  Definition HM2:=HybridMachine hb2 Sems Semt.
-
   Variable U: seq.seq nat.
 
   (*I use none, but it should be the initial memory. FIX. *)
-  Definition Sem1:=(ConcurMachineSemantics _ _ _ HM1 U None).
-  Definition Sem2:=(ConcurMachineSemantics _ _ _ HM2 U None) .
+  Definition HCSem Sems Semt hb U:=
+    (ConcurMachineSemantics _ _ _ (HybridMachine hb Sems Semt) U None).
+  Notation Sem1:= (HCSem Sems Semt hb1 U).
+  Notation Sem2:= (HCSem Sems Semt hb2 U).
   
   Notation C1:= (t_ (ThreadPool hb1 Sems Semt)).
   Notation C2:= (t_ (ThreadPool hb2 Sems Semt)).
-  Definition G:= (semG Sems * semG Semt)%type.
+  Notation G:= (semG Sems * semG Semt)%type.
   Variable ge:G.
-  Variable (ge_inv: G -> G -> Prop).
-
-  
-  Variable init_inv : meminj -> G -> list val -> mem -> G -> list val -> mem -> Prop.
-
-  Variable halt_inv : (*SM_Injection*)meminj -> G -> val -> mem -> G -> val -> mem -> Prop.
 
   Variable core_data: Type.
   Variable core_ord : core_data -> core_data -> Prop.
   Variable core_ord_wf : well_founded core_ord.
-  Variable thread_match : core_data -> (*SM_Injection*)meminj -> (semC Sems) -> mem -> (semC Semt) -> mem -> Prop.
-  Variable source_match : (*SM_Injection*)meminj -> (semC Sems) -> mem -> (semC Sems) -> mem -> Prop.
-  Variable target_match : (*SM_Injection*)meminj -> (semC Semt) -> mem -> (semC Semt) -> mem -> Prop.
-
+  
   Record HybridMachine_simulation
          (concur_match: core_data -> meminj -> C1 -> mem -> C2 -> mem -> Prop)
          main:=
-    { genv_inv : ge_inv ge ge
+    { Hybfsim_order_wf: well_founded core_ord
       ; core_initial :
           forall j c1 vals1 m1 vals2 m2,
             machine_semantics.initial_machine Sem1 ge main vals1 = Some c1 ->
-            init_inv j ge vals1 m1 ge vals2 m2 ->
-    exists (*mu*) cd c2,
-      (*as_inj mu = j*
-      /\*) machine_semantics.initial_machine Sem2 ge main vals2 = Some c2
+            exists cd c2,
+              machine_semantics.initial_machine Sem2 ge main vals2 = Some c2
            /\ concur_match cd j c1 m1 c2 m2
       ; thread_diagram :
           forall U st1 m1 st1' m1',
@@ -100,29 +88,174 @@ Section HybridSimulation.
               exists st2', exists m2', exists cd', exists mu',
                       concur_match cd' mu' st1' m1' st2' m2'
                       /\ (thread_step_plus Sem2 ge U st2 m2 st2' m2'
-               \/ (thread_step_star Sem2 ge U st2 m2 st2' m2' /\ core_ord cd' cd))
+                         \/ (thread_step_star Sem2 ge U st2 m2 st2' m2' /\ core_ord cd' cd))
       ; machine_diagram :
           forall U tr st1 m1 U' tr' st1' m1',
             machine_semantics.machine_step Sem1 ge U tr st1 m1 U' tr' st1' m1' ->
             forall cd st2 mu m2,
               concur_match cd mu st1 m1 st2 m2 ->
               exists st2', exists m2', exists cd',
-                      concur_match cd' mu st1' m1' st2' m2'
-                      /\ machine_semantics.machine_step Sem2 ge U tr st2 m2 U' tr' st2' m2'
+                    concur_match cd' mu st1' m1' st2' m2'
+                    /\ machine_semantics.machine_step Sem2 ge U tr st2 m2 U' tr' st2' m2'
       ; thread_halted :
           forall cd mu U c1 m1 c2 m2 v1,
             concur_match cd mu c1 m1 c2 m2 ->
             conc_halted Sem1 U c1 = Some v1 ->
-            exists j v2,
-              halt_inv j ge v1 m1 ge v2 m2
-              /\ conc_halted Sem2 U c2 = Some v2
+            exists v2,
+              conc_halted Sem2 U c2 = Some v2
       ; thread_running:
           forall cd mu c1 m1 c2 m2 ,
             concur_match cd mu c1 m1 c2 m2 ->
             forall i, runing_thread Sem1 c1 i <-> runing_thread Sem2 c2 i
             (* runing_thread Sem1 c1 = runing_thread Sem2 c2 *)
- }.
+    }.
+  
+End HybridSimulation.
+
+Inductive HM_forward_sim Sems Semt hb1 hb2 U G v:=
+| Build_HM_forward_sim: forall core_data core_order match_states,
+    HybridMachine_simulation Sems Semt hb1 hb2 U G
+                             core_data core_order match_states v ->
+    HM_forward_sim Sems Semt hb1 hb2 U G v.
+Section HybridListComposition.
+
+  
+  Variable (Sems Semt : Semantics_rec).
+  Variable (hb1 hb2 hb3: option nat).
+
+  Variable U: seq.seq nat.
+
+  (*I use none, but it should be the initial memory. FIX. *)
+  Notation Sem1:= (HCSem Sems Semt hb1 U).
+  Notation Sem2:= (HCSem Sems Semt hb2 U).
+  Notation Sem3:= (HCSem Sems Semt hb3 U).
+  
+  Notation C1:= (t_ (ThreadPool hb1 Sems Semt)).
+  Notation C2:= (t_ (ThreadPool hb2 Sems Semt)).
+  Notation C3:= (t_ (ThreadPool hb3 Sems Semt)).
+  Notation G:= (semG Sems * semG Semt)%type.
+  Variable ge:G.
+  
+  Variable data : Type.
+  Notation ls_data:=(list data).
+  Variable order: data -> data -> Prop.
+  Parameter ls_order : (data -> data -> Prop) -> list data -> list data -> Prop.
+  Parameter ls_ord_wf : forall order, well_founded order -> well_founded (ls_order order).
+  Notation ls_order':=(ls_order order).
+
+  Notation HybridMachine_simulation hb1 hb2:=
+    (HybridMachine_simulation Sems Semt hb1 hb2 U ge ).
+
+  Variable v:val.
+  
+  Variable (match12 : list data -> meminj -> C1 -> mem -> C2 -> mem -> Prop).
+  Hypothesis Hsimulation12:
+      HybridMachine_simulation hb1 hb2 ls_data ls_order' match12 v.
+
+  Variable (match23 : data -> meminj -> C2 -> mem -> C3 -> mem -> Prop).
+  Hypothesis Hsimulation23:
+      HybridMachine_simulation hb2 hb3 data order match23 v.
+
+  Definition ls_compose_match
+             (d123:list data)
+             (f:meminj)
+             (c1:C1) (m1:mem) (c3:C3)(m3:mem): Prop:= 
+    exists c2 m2 f12 f23,
+      exists d12 d23, d123 = d23::d12 /\
+      match12 d12 f12 c1 m1 c2 m2 /\
+      match23 d23 f23 c2 m2 c3 m3 /\
+      f = compose_meminj f12 f23.
+      
+  Lemma Hsim_ls_composition:
+    HybridMachine_simulation hb1 hb3
+                             ls_data
+                             ls_order'
+                             ls_compose_match v. 
+  Proof.
+    constructor.
+    - admit. (*wf of list order*)
+    - admit. (*Initial*)
+    - admit. (*Thread step*)
+    - intros ? ? ? ? ? tr3 ? ? ? ? st3 ? m3 ?.
+      destruct H0 as
+          (c2 & m2 & f12 & f23 & d12 & d23 & D & M12 & M23 & inj_comp).
+      eapply Hsimulation12 in H; eauto. 
+      destruct H as
+          (c2' & m2' & cd'' & M12' & STEP2).
+      eapply Hsimulation23 in STEP2; eauto.
+      destruct STEP2 as (c3' & m3' & cd3 & M23' & STEP3).
+      exists c3', m3', (cd3::cd''); split; eauto.
+      exists c2', m2', f12, f23, cd'', cd3; split; eauto.
+    - admit. (*Halted step*)
+    - admit. (*Running step*)
+  Admitted.
 
 
+End HybridListComposition.
 
-  End HybridSimulation.
+Section HybridComposition.
+
+  
+  Variable (Sems Semt : Semantics_rec).
+  Variable (hb1 hb2 hb3: option nat).
+
+  Variable U: seq.seq nat.
+
+  (*I use none, but it should be the initial memory. FIX. *)
+  Notation Sem1:= (HCSem Sems Semt hb1 U).
+  Notation Sem2:= (HCSem Sems Semt hb2 U).
+  Notation Sem3:= (HCSem Sems Semt hb3 U).
+  
+  Notation C1:= (t_ (ThreadPool hb1 Sems Semt)).
+  Notation C2:= (t_ (ThreadPool hb2 Sems Semt)).
+  Notation C3:= (t_ (ThreadPool hb3 Sems Semt)).
+  Notation G:= (semG Sems * semG Semt)%type.
+  Variable ge:G.
+  
+  Variable data12 data23: Type.
+  Variable ord12 : data12 -> data12 -> Prop.
+  Variable ord23 : data23 -> data23 -> Prop.
+  Variable ord_wf12 : well_founded ord12.
+  Variable ord_wf23 : well_founded ord23.
+
+  Notation HybridMachine_simulation hb1 hb2:=
+    (HybridMachine_simulation Sems Semt hb1 hb2 U ge ).
+
+  Variable v:val.
+  
+  Variable (match12 : data12 -> meminj -> C1 -> mem -> C2 -> mem -> Prop).
+  Hypothesis Hsimulation12:
+      HybridMachine_simulation hb1 hb2 data12 ord12 match12 v.
+
+  Variable (match23 : data23 -> meminj -> C2 -> mem -> C3 -> mem -> Prop).
+  Hypothesis Hsimulation23:
+      HybridMachine_simulation hb2 hb3 data23 ord23 match23 v.
+
+  Definition compose_match
+             (d123:data23 * data12)
+             (f:meminj)
+             (c1:C1) (m1:mem) (c3:C3)(m3:mem): Prop:= 
+    exists c2 m2 f12 f23, 
+      match12 (snd d123) f12 c1 m1 c2 m2 /\
+      match23 (fst d123) f23 c2 m3 c3 m3 /\
+      f = compose_meminj f12 f23.
+      
+  Lemma Hsim_composition:
+    HybridMachine_simulation hb1 hb3
+                             (data23 * data12)
+                             (lex_ord (clos_trans _ ord23) ord12)
+                             compose_match v. 
+  Proof.
+    constructor.
+    - apply wf_lex_ord. apply Transitive_Closure.wf_clos_trans.
+      eapply Hybfsim_order_wf; eauto.
+      eapply Hybfsim_order_wf; eauto.
+    - admit. (*Initial*)
+    - admit. (*Thread step*)
+    - admit. (*Machine step*)
+    - admit. (*Halted step*)
+    - admit. (*Running step*)
+  Admitted.
+
+
+End HybridComposition.
