concurrency/HybridMachine_simulation_proof.v
@@ -3,6 +3,7 @@ Require Import Coq.omega.Omega.
 Require Import Clight.
 Require Import Memory.
 Require Import Values.
+Require Import Globalenvs.
 Require Import Compiler.
 Require Import compcert.lib.Coqlib.
 
@@ -11,7 +12,7 @@ Require Import msl.Coqlib2.
 Require veric.Clight_core. Import Clight_core.
 
 Require Import Smallstep.
-Require Import ExposedSmallstep2.
+Require Import ExposedSmallstep2 ExposedSmallstep.
 Require Import concurrency.x86_context.
 Require Import concurrency.HybridMachine.
 Require Import concurrency.HybridMachineSig.
@@ -19,43 +20,15 @@ Require Import concurrency.HybridMachine_simulation.
 (*Require Import concurrency.compiler_correct.*)
 Require Import concurrency.CoreSemantics_sum.
 Require Import concurrency.self_simulation.
+Require Import concurrency.Clight_self_simulation.
+Require Import concurrency.Asm_self_simulation.
+
 
 Require Import concurrency.permissions.
 
+Require Import concurrency.ClightCoreSemantincsForMachines.
+
 Set Bullet Behavior "Strict Subproofs".
-
-
-
-Section Clight_Sem.
-  Variable p: program.
-  
-  Notation genv:=genv. (*from Clight_core*)
-  Notation state:=CC_core.
-  
-  Program Definition Clight_memSem: semantics.MemSem genv state:=
-    semantics.Build_MemSem _ _ cl_core_sem _.
-  Next Obligation.
-  Admitted.
-
-  Program Definition Clight_EvSem: event_semantics.EvSem:=
-    event_semantics.Build_EvSem _ _ Clight_memSem _ _ _ _ _.
-  Next Obligation.
-  Admitted.
-  Next Obligation.
-  Admitted.
-  Next Obligation.
-  Admitted.
-  Next Obligation.
-  Admitted.
-  Next Obligation.
-  Admitted.
-    
-  Definition Clight: Semantics_rec:=
-    Build_Semantics_rec
-      genv (*semG*)
-      state (*semC*)
-      Clight_EvSem (*semSem EvSem*).
-End Clight_Sem.
 
 Section HybridProofs.
 
@@ -63,63 +36,15 @@ Section HybridProofs.
   Variable tp: ia32.Asm.program. 
   Variable compiled: (simpl_transf_clight_program p = Errors.OK tp).
 
-  (*Lemma programs_match : simpl_match_prog p tp.
-  Proof. apply transf_clight_program_match; assumption. Qed.
-
-  Lemma program_forward_sim:
-    Smallstep.forward_simulation (semantics2 p) (Asm.semantics tp).
-  Proof. apply simpl_clight_semantic_preservation; apply programs_match; eauto. Qed. *)
-
-  Parameter Clight_step: Clight.genv -> CC_core * mem -> Events.trace -> CC_core * mem -> Prop.
-  Parameter Clight_init: CC_core * mem -> Prop.
-  Parameter Clight_final: CC_core * mem -> Integers.Int.int -> Prop.
-  Parameter Clight_genv: program -> Clight.genv.
-  Parameter Clight_symbolenv: Globalenvs.Senv.t.
   Definition Clight_semantics2 (p: program) : semantics:=
-    @Semantics_gen
-      (CC_core * mem)
-      Clight.genv
-      Clight_step
-      Clight_init
-      Clight_final
-      (Clight_genv p)
-      Clight_symbolenv.
-  Definition Clight_get_mem (cs: (CC_core * mem)):= match cs with ( _ , m ) => m end.
+    Clight.semantics2 p.
 
-  Parameter Clight_code_inject: CC_core -> meminj -> CC_core -> Prop.
-  Lemma Clight_self_simulation: self_simulation _ _ (event_semantics.msem (semSem (Clight p))) Clight_code_inject.
-  Admitted.
-
-  Notation ASM_core:=X86Machines.ErasedMachine.ThreadPool.code.
-  Parameter Asm_step: X86SEM.G -> ASM_core * mem -> Events.trace -> ASM_core * mem -> Prop.
-  Parameter Asm_init: ASM_core * mem -> Prop.
-  Parameter Asm_final: ASM_core * mem -> Integers.Int.int -> Prop.
-  Parameter Asm_genv: ia32.Asm.program -> X86SEM.G.
-  Parameter Asm_symbolenv: Globalenvs.Senv.t.
-  Definition Asm_semantics (tp: ia32.Asm.program) : semantics:=
-    @Semantics_gen
-      (X86Machines.ErasedMachine.ThreadPool.code * mem)
-      X86SEM.G
-      Asm_step
-      Asm_init
-      Asm_final
-      (Asm_genv tp)
-      Asm_symbolenv.
-  Definition Asm_get_mem (cs: (X86Machines.ErasedMachine.ThreadPool.code  * mem)):= match cs with ( _ , m ) => m end.
-
-  Parameter Asm_code_inject: ASM_core -> meminj -> ASM_core -> Prop.
-  Lemma Asm_self_simulation: self_simulation _ _
-                                             (event_semantics.msem (semSem (X86SEM_rec)))
-                                             Asm_code_inject.
-  Admitted.
+  Definition Asm_semantics (tp: Asm.program) : semantics:=
+    Asm.semantics tp.
 
   
-  Lemma program_forward_sim:
-    forward_injection (Clight_semantics2 p) (Asm_semantics tp) Clight_get_mem Asm_get_mem.
-  Proof. Admitted.
-
-  Definition Sems:= Clight p.
-  Definition Semt:= X86SEM_rec.  (*How do I pass p to this?*)
+  Definition Sems:= ClightSEM_rec.
+  Definition Semt:= X86SEM_rec. 
 
 
 Section OneThreadCompiled.
@@ -127,10 +52,6 @@ Section OneThreadCompiled.
   Notation hb1:= (Some hb').
   Notation hb2:= (Some (S hb')).
   Variable U: seq.seq nat.
-
-  (* Definition Resources : Resources_rec:=
-    Build_Resources_rec (access_map * access_map)%type (access_map * access_map)%type. *)
-
   
   Notation C1:= (t_ (HybridMachine.ThreadPool hb1 Sems Semt)).
   Notation C2:= (t_ (HybridMachine.ThreadPool hb2 Sems Semt)).
@@ -138,192 +59,182 @@ Section OneThreadCompiled.
   Notation G2:= (semG (HybridMachine.Sem hb2 Sems Semt)).
 
   (*The two following globals must be taken from the program...*)
+
+
   (*and they are probaly the smae global??? *)
-  Variable genv: (semG Sems * semG Semt)%type.
+  Definition genvS:= Clight.globalenv p.
+  Definition genvT:= (Genv.globalenv tp).
+  Definition genv:= (genvS, genvT).
 
-
-  (*What are these!!!*)
-  Variable (ge_inv: G1 -> G2 -> Prop).
-  Variable init_inv : meminj -> G1 -> list val -> mem -> G2 -> list val -> mem -> Prop.
-  Variable halt_inv : (*SM_Injection*)meminj -> G1 -> val -> mem -> G2 -> val -> mem -> Prop.
   
   Section OneThreadCompiledProofs.
-  Definition match_source:= match_self (semC (Clight p)) Clight_code_inject.
-  Definition match_target:= match_self (semC (X86SEM_rec)) Asm_code_inject.
-  Definition make_state_source (c:semC Sems) (m:mem): state (Clight_semantics2 p):= (c, m).
-  Definition make_state_target (c:semC Semt) (m:mem): state (Asm_semantics tp):= (c,m).
-  Definition match_states {core_data: Type}
-             (compiler_match : core_data -> meminj -> state (Clight_semantics2 p)  -> state (Asm_semantics tp) -> Prop):=
-      fun i j c m c' m' => compiler_match i j (make_state_source c m) (make_state_target c' m').
+
+    (* we extract match_source from the self_simulation of Clight*)
+    Definition code_inject_source:= code_inject _ _ (Clight_self_simulation p).
+
+    (* we extract match_target from the self_simulation of Asm*)
+    Definition code_inject_target:= code_inject _  _ (Asm_self_simulation tp).
+
+    Parameter make_state_Clight: CC_core -> mem -> Clight.state.
+    Parameter make_state_Asm: X86Machines.ErasedMachine.ThreadPool.code -> mem -> ia32.Asm.state.
+
     
-  
-  
+    Definition compiler_simulation: fsim_properties_inj ( Clight.semantics2 p) (ia32.Asm.semantics tp)
+                                                        ( Clight.get_mem) (ia32.Asm.get_mem):=
+    simpl_clight_semantic_preservation p tp compiled.
+    
+    Definition compiler_index := Injindex compiler_simulation.
+    Definition compiler_order := Injorder compiler_simulation.
+    Definition compiler_match := Injmatch_states compiler_simulation.
+    
+    Definition match_compiled_states :=
+      fun i f c1 m1 c2 m2 =>
+        exists st1 st2 f1 f12 f2,
+          code_inject_source f1 (make_state_Clight c1 m1) st1 /\
+          compiler_match i f12 st1 st2 /\
+          code_inject_target f2 (make_state_Asm c2 m2) st2 /\
+          f = compose_meminj f1 (compose_meminj f12 f2).
+    Definition source_match f st1 m1 st2 m2 :=
+      code_inject_source f (make_state_Clight st1 m1)
+                         (make_state_Clight st2 m2).
+    Definition target_match f st1 m1 st2 m2 :=
+      code_inject_target f (make_state_Asm st1 m1)
+                         (make_state_Asm st2 m2).
+          
 Section OneThreadCompiledMatch.
 
-  Variable (Sems Semt : Semantics_rec).
   Definition HM1:=HybridMachine hb1 Sems Semt.
   Definition HM2:=HybridMachine hb2 Sems Semt.
 
   Notation Sem1:=(ConcurMachineSemantics _ _ _ HM1 U None).
   Notation Sem2:=(ConcurMachineSemantics _ _ _ HM2 U None) .
 
-  Notation C1:= (t_ (ThreadPool hb1 Sems Semt)).
-  Notation C2:= (t_ (ThreadPool hb2 Sems Semt)).
-  Definition G:= (semG Sems * semG Semt)%type.
+  Inductive condition: Set :=
+    running | blocked | resuming | initializing .
 
-  
-  Variable ge:G.
-  Variable (ge_inv': G -> G -> Prop).
-
-  (*
-  Variable init_inv' : meminj -> G -> list val -> mem -> G -> list val -> mem -> Prop.
-  Variable halt_inv' : (*SM_Injection*)meminj -> G -> val -> mem -> G -> val -> mem -> Prop.
-   *)
-  
-  Variable core_data: Type.
-  Variable core_ord : core_data -> core_data -> Prop.
-  Variable core_ord_wf : well_founded core_ord.
-  Variable thread_match : core_data -> (*SM_Injection*)meminj -> (semC Sems) -> mem -> (semC Semt) -> mem -> Prop.
-  Variable source_match : (*SM_Injection*)meminj -> (semC Sems) -> mem -> (semC Sems) -> mem -> Prop.
-  Variable target_match : (*SM_Injection*)meminj -> (semC Semt) -> mem -> (semC Semt) -> mem -> Prop.
-
-  Variable compiler_match : core_data -> meminj -> semC Sems -> mem -> semC Semt -> mem -> Prop.
-  
-Definition order_option (d1 d2: (option core_data)):=
-  match d1, d2 with
-  | None, None => True
-  | None, _ => True
-  | Some d1', Some d2' => core_ord d1' d2'
-  | _, _ => False
-  end.
-Fixpoint core_ord_list (ls1 ls2: list (option core_data)): Prop:=
-    match ls1, ls2 with
-    | nil, nil => True
-    | d1::ls1',d2::ls2' => order_option d1 d2 /\ core_ord_list ls1' ls2' 
-    | _, _ => False
+  Definition get_condition {cT} (c:@ctl cT):=
+    match c with
+    | Krun _ => running
+    | Kblocked _ => blocked
+    | Kresume _ _ => resuming
+    | Kinit _ _ =>  initializing
     end.
 
-Inductive condition: Set :=
-  running | blocked | resuming | initializing .
+  Definition get_state_inside {cT} (c:@ctl cT):=
+    match c with
+    | Krun c => Some c
+    | Kblocked c => Some c
+    | Kresume c _ => Some c
+    | Kinit _ _ =>  None
+    end.
 
-Definition get_condition {cT} (c:@ctl cT):=
-match c with
-| Krun _ => running
-| Kblocked _ => blocked
-| Kresume _ _ => resuming
-| Kinit _ _ =>  initializing
-end.
+  (*This will probably need reworking*)
 
-Definition get_state_inside {cT} (c:@ctl cT):=
-match c with
-| Krun c => Some c
-| Kblocked c => Some c
-| Kresume c _ => Some c
-| Kinit _ _ =>  None
-end.
+  Lemma same_length_contains:
+    forall {ms1: C1} {ms2: C2} {i},
+      num_threads ms1 = num_threads ms2 ->
+      containsThread ms1 i ->
+      containsThread ms2 i.
+  Proof.
+    intros ? ? ? H; unfold containsThread.
+    rewrite H; trivial.
+  Qed.
+  
+  Notation CoreSem Sem :=(semantics.csem(event_semantics.msem (semSem Sem))).
 
-(*This will probably need reworking*)
-
-Lemma same_length_contains:
-  forall {ms1: C1} {ms2: C2} {i},
-    num_threads ms1 = num_threads ms2 ->
-    containsThread ms1 i ->
-    containsThread ms2 i.
-Proof.
-  intros ? ? ? H; unfold containsThread.
-  rewrite H; trivial.
-Qed.
-
-Notation CoreSem Sem :=(semantics.csem(event_semantics.msem (semSem Sem))).
-
-Inductive match_thread_source (source_match: meminj -> (semC Sems) -> mem -> (semC Sems) -> mem -> Prop):
-  meminj -> @ctl (state_sum (semC Sems) (semC Semt)) -> mem -> @ctl (state_sum (semC Sems) (semC Semt)) -> mem -> Prop  :=
-| SThread_Running: forall j code1 m1 code2 m2,
-                     source_match j code1 m1 code2 m2 ->
-                     match_thread_source source_match j (Krun (SState _ _ code1)) m1
-                     (Krun (SState _ _ code2)) m2
-| SThread_Blocked: forall j code1 m1 code2 m2 ls1 ls2 f f',
-    semantics.at_external (CoreSem Sems) code1 = Some (f,ls1) ->
-    semantics.at_external (CoreSem Sems) code2 = Some (f',ls2) ->
-    Val.inject_list j ls1 ls2 ->
-    source_match j code1 m1 code2 m2 ->
-    match_thread_source source_match j (Kblocked (SState _ _ code1)) m1
-                        (Kblocked (SState _ _ code2)) m2
-| SThread_Resume: forall j code1 m1 code2 m2 ls1 ls2 f f' v v' code1' code2',
-    (*Do I need to keep this two? Probanly not*)
+  Inductive match_thread_source:
+    meminj -> @ctl (state_sum (semC Sems) (semC Semt)) -> mem -> @ctl (state_sum (semC Sems) (semC Semt)) -> mem -> Prop  :=
+  | SThread_Running: forall j code1 m1 code2 m2,
+      source_match j code1 m1 code2 m2 ->
+      match_thread_source
+        j (Krun (SState _ _ code1)) m1
+        (Krun (SState _ _ code2)) m2
+  | SThread_Blocked: forall j code1 m1 code2 m2 ls1 ls2 f f',
+      semantics.at_external (CoreSem Sems) code1 = Some (f,ls1) ->
+      semantics.at_external (CoreSem Sems) code2 = Some (f',ls2) ->
+      Val.inject_list j ls1 ls2 ->
+      source_match j code1 m1 code2 m2 ->
+      match_thread_source  j (Kblocked (SState _ _ code1)) m1
+                          (Kblocked (SState _ _ code2)) m2
+  | SThread_Resume: forall j code1 m1 code2 m2 ls1 ls2 f f' v v' code1' code2',
+      (*Do I need to keep this two? Probanly not*)
     semantics.at_external (CoreSem Sems) code1 = Some (f,ls1) ->
     semantics.at_external (CoreSem Sems) code2 = Some (f',ls2) ->
     Val.inject_list j ls1 ls2 ->
     semantics.after_external (CoreSem Sems) None code1 = Some code1' ->
     semantics.after_external (CoreSem Sems) None code2 = Some code2' ->
     source_match j code1' m2 code2' m2 ->
-    match_thread_source source_match j (Kresume (SState _ _ code1) v) m1
+    match_thread_source j (Kresume (SState _ _ code1) v) m1
                         (Kresume (SState _ _ code2) v') m2
 | SThread_Init: forall j m1 m2 v1 v1' v2 v2',
     Val.inject j v1 v2 ->
     Val.inject j v1' v2' ->
-    match_thread_source source_match j (Kinit v1 v1') m1
+    match_thread_source j (Kinit v1 v1') m1
                         (Kinit v2 v2') m2.
 
-Inductive match_thread_target (target_match: meminj -> (semC Semt) -> mem -> (semC Semt) -> mem -> Prop):
-  meminj -> @ctl (state_sum (semC Sems) (semC Semt)) -> mem -> @ctl (state_sum (semC Sems) (semC Semt)) -> mem -> Prop  :=
-| TThread_Running: forall j code1 m1 code2 m2,
-                     target_match j code1 m1 code2 m2 ->
-                     match_thread_target target_match j (Krun (TState _ _ code1)) m1
-                     (Krun (TState _ _ code2)) m2
-| TThread_Blocked: forall j code1 m1 code2 m2 ls1 ls2 f f',
-    semantics.at_external (CoreSem Semt) code1 = Some (f,ls1) ->
-    semantics.at_external (CoreSem Semt) code2 = Some (f',ls2) ->
-    Val.inject_list j ls1 ls2 ->
-    target_match j code1 m1 code2 m2 ->
-    match_thread_target target_match j (Kblocked (TState _ _ code1)) m1
-                        (Kblocked (TState _ _ code2)) m2
-| TThread_Resume: forall j code1 m1 code2 m2 ls1 ls2 f f' v v' code1' code2',
-    (*Do I need to keep this two? Probanly not*)
-    semantics.at_external (CoreSem Semt) code1 = Some (f,ls1) ->
-    semantics.at_external (CoreSem Semt) code2 = Some (f',ls2) ->
-    Val.inject_list j ls1 ls2 ->
-    semantics.after_external (CoreSem Semt) None code1 = Some code1' ->
-    semantics.after_external (CoreSem Semt) None code2 = Some code2' ->
-    target_match j code1' m2 code2' m2 ->
-    match_thread_target target_match j (Kresume (TState _ _ code1) v) m1
-                        (Kresume (TState _ _ code2) v') m2
-| TThread_Init: forall j m1 m2 v1 v1' v2 v2',
-    Val.inject j v1 v2 ->
-    Val.inject j v1' v2' ->
-    match_thread_target target_match j (Kinit v1 v1') m1
-                        (Kinit v2 v2') m2.
+  Inductive match_thread_target :
+    meminj -> @ctl (state_sum (semC Sems) (semC Semt)) -> mem -> @ctl (state_sum (semC Sems) (semC Semt)) -> mem -> Prop  :=
+  | TThread_Running: forall j code1 m1 code2 m2,
+      target_match j code1 m1 code2 m2 ->
+      match_thread_target  j (Krun (TState _ _ code1)) m1
+                          (Krun (TState _ _ code2)) m2
+  | TThread_Blocked: forall j code1 m1 code2 m2 ls1 ls2 f f',
+      semantics.at_external (CoreSem Semt) code1 = Some (f,ls1) ->
+      semantics.at_external (CoreSem Semt) code2 = Some (f',ls2) ->
+      Val.inject_list j ls1 ls2 ->
+      target_match j code1 m1 code2 m2 ->
+      match_thread_target j (Kblocked (TState _ _ code1)) m1
+                          (Kblocked (TState _ _ code2)) m2
+  | TThread_Resume: forall j code1 m1 code2 m2 ls1 ls2 f f' v v' code1' code2',
+      (*Do I need to keep this two? Probanly not*)
+      semantics.at_external (CoreSem Semt) code1 = Some (f,ls1) ->
+      semantics.at_external (CoreSem Semt) code2 = Some (f',ls2) ->
+      Val.inject_list j ls1 ls2 ->
+      semantics.after_external (CoreSem Semt) None code1 = Some code1' ->
+      semantics.after_external (CoreSem Semt) None code2 = Some code2' ->
+      target_match j code1' m2 code2' m2 ->
+      match_thread_target j (Kresume (TState _ _ code1) v) m1
+                          (Kresume (TState _ _ code2) v') m2
+  | TThread_Init: forall j m1 m2 v1 v1' v2 v2',
+      Val.inject j v1 v2 ->
+      Val.inject j v1' v2' ->
+      match_thread_target j (Kinit v1 v1') m1
+                          (Kinit v2 v2') m2.
 
-Inductive match_thread_compiled (compiler_match: meminj -> (semC Sems) -> mem -> (semC Semt) -> mem -> Prop):
-  meminj -> @ctl (state_sum (semC Sems) (semC Semt)) -> mem -> @ctl (state_sum (semC Sems) (semC Semt)) -> mem -> Prop  :=
-| CThread_Running: forall j code1 m1 code2 m2,
-                     compiler_match j code1 m1 code2 m2 ->
-                     match_thread_compiled compiler_match j (Krun (SState _ _ code1)) m1
-                     (Krun (TState _ _ code2)) m2
-| CThread_Blocked: forall j code1 m1 code2 m2 ls1 ls2 f f',
-    semantics.at_external (CoreSem Sems) code1 = Some (f,ls1) ->
-    semantics.at_external (CoreSem Semt) code2 = Some (f',ls2) ->
-    Val.inject_list j ls1 ls2 ->
-    compiler_match j code1 m1 code2 m2 ->
-    match_thread_compiled compiler_match j (Kblocked (SState _ _ code1)) m1
-                        (Kblocked (TState _ _ code2)) m2
-| CThread_Resume: forall j code1 m1 code2 m2 ls1 ls2 f f' v v' code1' code2',
-    (*Do I need to keep this two? Probanly not*)
-    semantics.at_external (CoreSem Sems) code1 = Some (f,ls1) ->
-    semantics.at_external (CoreSem Semt) code2 = Some (f',ls2) ->
-    Val.inject_list j ls1 ls2 ->
-    semantics.after_external (CoreSem Sems) None code1 = Some code1' ->
-    semantics.after_external (CoreSem Semt) None code2 = Some code2' ->
-    compiler_match j code1' m1 code2' m2 ->
-    match_thread_compiled compiler_match j (Kresume (SState _ _ code1) v) m1
-                        (Kresume (TState _ _ code2) v') m2
-| CThread_Init: forall j m1 m2 v1 v1' v2 v2',
-    Val.inject j v1 v2 ->
-    Val.inject j v1' v2' ->
-    match_thread_compiled compiler_match j (Kinit v1 v1') m1
-                        (Kinit v2 v2') m2.
+  (* match_compiled_states *)
+  
+  Inductive match_thread_compiled:
+    compiler_index -> meminj ->
+    @ctl (state_sum (semC Sems) (semC Semt)) -> mem ->
+    @ctl (state_sum (semC Sems) (semC Semt)) -> mem -> Prop  :=
+  | CThread_Running: forall cd j code1 m1 code2 m2,
+      match_compiled_states cd j code1 m1 code2 m2 ->
+      match_thread_compiled cd j (Krun (SState _ _ code1)) m1
+                            (Krun (TState _ _ code2)) m2
+  | CThread_Blocked: forall cd j code1 m1 code2 m2 ls1 ls2 f f',
+      semantics.at_external (CoreSem Sems) code1 = Some (f,ls1) ->
+      semantics.at_external (CoreSem Semt) code2 = Some (f',ls2) ->
+      Val.inject_list j ls1 ls2 ->
+      match_compiled_states cd j code1 m1 code2 m2 ->
+      match_thread_compiled  cd j (Kblocked (SState _ _ code1)) m1
+                            (Kblocked (TState _ _ code2)) m2
+  | CThread_Resume: forall cd j code1 m1 code2 m2 ls1 ls2 f f' v v' code1' code2',
+      (*Do I need to keep this two? Probanly not*)
+      semantics.at_external (CoreSem Sems) code1 = Some (f,ls1) ->
+      semantics.at_external (CoreSem Semt) code2 = Some (f',ls2) ->
+      Val.inject_list j ls1 ls2 ->
+      semantics.after_external (CoreSem Sems) None code1 = Some code1' ->
+      semantics.after_external (CoreSem Semt) None code2 = Some code2' ->
+      match_compiled_states cd j code1' m1 code2' m2 ->
+      match_thread_compiled cd j (Kresume (SState _ _ code1) v) m1
+                            (Kresume (TState _ _ code2) v') m2
+  | CThread_Init: forall cd j m1 m2 v1 v1' v2 v2',
+      Val.inject j v1 v2 ->
+      Val.inject j v1' v2' ->
+      match_thread_compiled cd j (Kinit v1 v1') m1
+                            (Kinit v2 v2') m2.
 
-Record concur_match (index: core_data)
+  Record concur_match (cd: compiler_index)
        (j:meminj) (cstate1: C1) (m1: mem) (cstate2: C2) (m2: mem):=
   { same_length: num_threads cstate1 = num_threads cstate2
     ; memcompat1: HybridMachine.mem_compatible _ _ _ cstate1 m1
@@ -332,7 +243,7 @@ Record concur_match (index: core_data)
         forall (i:nat),
           (i > hb')%nat ->
           forall (cnti1: containsThread cstate1 i),
-          match_thread_source (source_match) j
+          match_thread_source  j
                               (getThreadC cnti1)
                               (restrPermMap (memcompat1 i cnti1).1)
                               (getThreadC (same_length_contains same_length cnti1))
@@ -341,7 +252,7 @@ Record concur_match (index: core_data)
         forall (i:nat),
           (i < hb')%nat ->
           forall (cnti1: containsThread cstate1 i),
-          match_thread_target (target_match) j
+          match_thread_target  j
                               (getThreadC cnti1)
                               (restrPermMap (memcompat1 i cnti1).1)
                               (getThreadC (same_length_contains same_length cnti1))
@@ -350,11 +261,11 @@ Record concur_match (index: core_data)
         forall (i:nat),
           (i = hb')%nat ->
           forall (cnti1: containsThread cstate1 i),
-          match_thread_compiled (compiler_match index) j
-                              (getThreadC cnti1)
-                              (restrPermMap (memcompat1 i cnti1).1)
-                              (getThreadC (same_length_contains same_length cnti1))
-                              (restrPermMap (memcompat2 i (same_length_contains same_length cnti1)).1) }.
+          match_thread_compiled cd j
+                                (getThreadC cnti1)
+                                (restrPermMap (memcompat1 i cnti1).1)
+                                (getThreadC (same_length_contains same_length cnti1))
+                                (restrPermMap (memcompat2 i (same_length_contains same_length cnti1)).1) }.
 
 Lemma contains12:
   forall {data j cstate1 m1 cstate2 m2},
@@ -380,15 +291,13 @@ Qed.
 
 End OneThreadCompiledMatch.
 
-Arguments same_length_contains {Sems Semt ms1 ms2 }.
-Arguments memcompat1 {Sems Semt core_data source_match target_match compiler_match index j cstate1 m1 cstate2 m2}.
-Arguments memcompat2 {Sems Semt core_data source_match target_match compiler_match index j cstate1 m1 cstate2 m2}.
-Arguments contains12 {Sems Semt core_data source_match target_match compiler_match data j cstate1 m1 cstate2 m2} _ {i}.
-Arguments contains21 {Sems Semt core_data source_match target_match compiler_match data j cstate1 m1 cstate2 m2} _ {i}.
-
+Arguments same_length_contains {ms1 ms2}.
+Arguments memcompat1 {cd j cstate1 m1 cstate2 m2}.
+Arguments memcompat2 {cd j cstate1 m1 cstate2 m2}.
     
   Section HybridThreadDiagram.
-    
+
+    (*
     Variable core_data : Type.
     Variable order : core_data -> core_data -> Prop.
     Variable compiler_match : core_data -> meminj -> state (Clight_semantics2 p)  -> state (Asm_semantics tp) -> Prop.
@@ -396,17 +305,21 @@ Arguments contains21 {Sems Semt core_data source_match target_match compiler_mat
                                          Clight_get_mem Asm_get_mem order compiler_match.
     Notation match_states:=(match_states compiler_match).
     Notation concur_match:=(@concur_match Sems Semt core_data match_source match_target match_states).
-    
+     *)
+
+    (*
     Lemma hybrid_thread_diagramc:
       forall (U0 : list nat) (st1 : C1) (m1 : mem) (st1' : C1) (m1' : mem),
-        machine_semantics.thread_step (Sem1 Sems Semt hb1 U) genv U0 st1 m1 st1' m1' ->
-        forall (cd : core_data) (st2 : C2) (mu : meminj) (m2 : mem),
+        machine_semantics.thread_step (HCSem Sems Semt hb1 U) genv U0 st1 m1 st1' m1' ->
+        forall cd (st2 : C2) (mu : meminj) (m2 : mem),
           concur_match cd mu st1 m1 st2 m2 ->
-          exists (st2' : C2) (m2' : mem) (cd' : core_data) (mu' : meminj),
+          exists (st2' : C2) (m2' : mem) cd' (mu' : meminj),
             concur_match cd' mu' st1' m1' st2' m2' /\
-            (machine_semantics_lemmas.thread_step_plus (Sem2 Sems Semt hb2 U) genv U0 st2 m2 st2' m2' \/
-     machine_semantics_lemmas.thread_step_star (Sem2 Sems Semt hb2 U) genv U0 st2 m2 st2' m2' /\
-             order cd' cd).
+            (machine_semantics_lemmas.thread_step_plus
+               (HCSem Sems Semt hb2 U) genv U0 st2 m2 st2' m2' \/
+             machine_semantics_lemmas.thread_step_star
+               (HCSem Sems Semt hb2 U) genv U0 st2 m2 st2' m2'
+             /\ compiler_order cd' cd).
     Proof.
       intros.
       destruct U0; simpl in H.
@@ -617,29 +530,21 @@ Arguments contains21 {Sems Semt core_data source_match target_match compiler_mat
         Unshelve.
         eauto.
         eauto.
-    Admitted.
+    Admitted. *)
     
-    End HybridThreadDiagram.
+  End HybridThreadDiagram.
 
   Section MachineThreadDiagram.
     
-    Variable core_data : Type.
-    Variable order : core_data -> core_data -> Prop.
-    Variable compiler_match : core_data -> meminj -> state (Clight_semantics2 p)  -> state (Asm_semantics tp) -> Prop.
-    Variable props : fsim_properties_inj (Clight_semantics2 p) (Asm_semantics tp)
-                                         Clight_get_mem Asm_get_mem order compiler_match.
-    Notation match_states:=(match_states compiler_match).
-    Notation concur_match:=(@concur_match Sems Semt core_data match_source match_target match_states).
-
-    Lemma machine_thread_diagram:
+    (*Lemma machine_thread_diagram:
       forall (U0 : list nat) (tr : list HybridMachineSig.machine_event) (st1 : C1) (m1 : mem) 
         (U' : list nat) (tr' : list HybridMachineSig.machine_event) (st1' : C1) (m1' : mem),
-        machine_semantics.machine_step (Sem1 Sems Semt hb1 U) genv U0 tr st1 m1 U' tr' st1' m1' ->
+        machine_semantics.machine_step (HCSem Sems Semt hb1 U) genv U0 tr st1 m1 U' tr' st1' m1' ->
         forall (cd : core_data) (st2 : C2) (mu : meminj) (m2 : mem),
           concur_match cd mu st1 m1 st2 m2 ->
           exists (st2' : C2) (m2' : mem) (cd' : core_data),
             concur_match cd' mu st1' m1' st2' m2' /\
-            machine_semantics.machine_step (Sem2 Sems Semt hb2 U) genv U0 tr st2 m2 U' tr' st2' m2'.
+            machine_semantics.machine_step (HCSem Sems Semt hb2 U) genv U0 tr st2 m2 U' tr' st2' m2'.
     Proof.
       intros.
       destruct U0; simpl in H.
@@ -662,30 +567,28 @@ Arguments contains21 {Sems Semt core_data source_match target_match compiler_mat
           admit.
         * (*schedfail'*)
           admit.
-    Admitted.
+    Admitted. *)
     
   End MachineThreadDiagram.
 
   (** *The one_compiled_thread_simulation*)
+
+  (*Fake genv while we fix Asm*)
+  Parameter genv':(semG Sems * semG Semt)%type.
+    
   Lemma one_compiled_thread_simulation:
-    exists (core_data: Type), exists (core_ord : core_data -> core_data -> Prop),
-        exists compiler_match, exists v:val,
+    exists v:val,
             HybridMachine_simulation
-              Sems Semt hb1 hb2 U genv ge_inv init_inv halt_inv
-              core_data core_ord
-              (concur_match _ _ core_data match_source
-                            match_target compiler_match)  v.
+              Sems Semt hb1 hb2 U genv'
+              _ compiler_order
+              (concur_match)  v.
   Proof.
-  pose proof program_forward_sim as HH.
-  inversion HH.
-  exists (index).
-  exists (order).
-  exists (match_states match_states0).
-  exists Vundef. (*THIS SHOULD DISAPEAR*)
-  constructor.
-  - (*ge_inv*)
-    admit.
+    
+  exists Vundef.
+  econstructor.
+  - eapply Injfsim_order_wf.
   - (* core_initial*)
+    intros.
     (* intros.
     simpl in H.
     destruct (
@@ -697,11 +600,12 @@ Arguments contains21 {Sems Semt core_data source_match target_match compiler_mat
     unfold HybridMachine.init_mach in INIT.  *)
     admit.
   - (*thread_diagram*)
-    eapply hybrid_thread_diagramc; eauto.
+    admit.
+    (* eapply hybrid_thread_diagramc; eauto. *)
     
   - (*machine_diagram*)
-    eapply machine_thread_diagram; eauto.
-
+    (* eapply machine_thread_diagram; eauto. *)
+    admit.
   - (*thread_halted *)
     admit.
     
@@ -714,46 +618,47 @@ End OneThreadCompiledProofs.
 End OneThreadCompiled.
 
 Section NThredCompiled.
-  Variable (hb': nat).
   Notation hb0:= (Some 0%nat).
-  Notation hbn:= (Some hb').
+  Notation hb n:= (Some n).
   Variable U: seq.seq nat.
 
   Notation C0:= (t_ (HybridMachine.ThreadPool hb0 Sems Semt)).
-  Notation Cn:= (t_ (HybridMachine.ThreadPool hbn Sems Semt)).
-  Notation G0:= (semG (HybridMachine.Sem hb0 Sems Semt)) .
-  Notation Gn:= (semG (HybridMachine.Sem hbn Sems Semt)).
+  Notation C n:= (t_ (HybridMachine.ThreadPool (Some n) Sems Semt)).
+  Notation G:= (semG (HybridMachine.Sem hb0 Sems Semt)) .
+  (*Notation G n:= (semG (HybridMachine.Sem (hb n) Sems Semt)). *)
 
-  (*The two following globals must be taken from the program...*)
-  (*and they are probaly the smae global??? *)
-  Variable genv: (semG Sems * semG Semt)%type.
-  
-  (*What are these!!!*)
-  Variable (ge_inv: G0 -> Gn -> Prop).
-  Variable init_inv : meminj -> G0 -> list val -> mem -> Gn -> list val -> mem -> Prop.
-  Variable halt_inv : (*SM_Injection*)meminj -> G0 -> val -> mem -> Gn -> val -> mem -> Prop.
 
-  Variable source_match : (*SM_Injection*)meminj -> (semC Sems) -> mem -> (semC Sems) -> mem -> Prop.
-  Variable target_match : (*SM_Injection*)meminj -> (semC Semt) -> mem -> (semC Semt) -> mem -> Prop.
-  
-  Definition Nconcur_match':
-    (meminj -> semC Sems -> mem -> semC Sems -> mem -> Prop) ->
-    (meminj -> semC Semt -> mem -> semC Semt -> mem -> Prop) ->
-    forall (core_data: Type) (core_ord:core_data -> core_data -> Prop),
-    (core_data -> meminj -> semC Sems -> mem -> semC Semt -> mem -> Prop) ->
-    core_data -> meminj -> C0 -> mem -> Cn -> mem -> Prop.
-  Admitted. 
+  (*Need to make the data/order correct: that is a list of cds'*)
+  Inductive  Nconcur_match: forall n, list compiler_index -> meminj -> C0 -> mem -> C n -> mem -> Prop :=
+  | ZeroOneSimulation:
+      forall st0 m0,
+        Nconcur_match 0 nil inject_id st0 m0 st0 m0
+  | ZeroNSimulation:
+      forall n ls_cd cd jn jn' st0 m0 stn mn stn' mn',
+        Nconcur_match n ls_cd jn st0 m0 stn mn ->
+        concur_match n cd jn' stn mn stn' mn' ->
+        Nconcur_match (S n) (cd::ls_cd) (compose_meminj jn jn') st0 m0 stn' mn'.
 
-  Notation Nconcur_match:=(Nconcur_match' match_source match_target).
-  
+  Parameter list_order: list compiler_index -> list compiler_index -> Prop.
+
+  Variable v:val.
   Lemma N_compiled_thread_simulation:
-    exists (core_data: Type), exists (core_ord : core_data -> core_data -> Prop),
-      exists compiler_match, exists v:val,
+    forall n,
           HybridMachine_simulation
-            Sems Semt hb0 hbn U genv ge_inv init_inv halt_inv
-            core_data core_ord 
-            (Nconcur_match core_data core_ord (match_states compiler_match))  v.  
+            Sems Semt hb0 (hb n) U genv'
+            (list compiler_index) list_order 
+            (Nconcur_match n)  v.  
   Proof.
+    induction n.
+    - simpl.
+      admit. (*Trivial self simulation.*)
+    - econstructor.
+      + admit.
+      + admit. (*init*)
+      + admit. (* regular composition diagram (needs the star lemma... ) *)
+      + admit. (* easy one step machine diagram *)
+      + admit. (* haltd*)
+      + admit.
   Admitted.
   
 End NThredCompiled.
@@ -765,39 +670,23 @@ Section AllThredCompiled.
   Variable U: seq.seq nat.
 
   Notation C0:= (t_ (HybridMachine.ThreadPool hb0 Sems Semt)).
-  Notation Cn:= (t_ (HybridMachine.ThreadPool hball Sems Semt)).
+  Notation Call:= (t_ (HybridMachine.ThreadPool hball Sems Semt)).
   Notation G0:= (semG (HybridMachine.Sem hb0 Sems Semt)) .
-  Notation Gn:= (semG (HybridMachine.Sem hball Sems Semt)).
+  Notation Gall:= (semG (HybridMachine.Sem hball Sems Semt)).
 
-  (*The two following globals must be taken from the program...*)
-  (*and they are probaly the smae global??? *)
-  Variable genv: (semG Sems * semG Semt)%type.
-  
-  (*What are these!!!*)
-  Variable (ge_inv: G0 -> Gn -> Prop).
-  Variable init_inv : meminj -> G0 -> list val -> mem -> Gn -> list val -> mem -> Prop.
-  Variable halt_inv : (*SM_Injection*)meminj -> G0 -> val -> mem -> Gn -> val -> mem -> Prop.
-
-  Variable source_match : (*SM_Injection*)meminj -> (semC Sems) -> mem -> (semC Sems) -> mem -> Prop.
-  Variable target_match : (*SM_Injection*)meminj -> (semC Semt) -> mem -> (semC Semt) -> mem -> Prop.
-  
+  (*Remember to use (match_states compiler_match) insted of compiler_match directly*)
   Definition All_concur_match':
-    (meminj -> semC Sems -> mem -> semC Sems -> mem -> Prop) ->
-    (meminj -> semC Semt -> mem -> semC Semt -> mem -> Prop) ->
-    forall (core_data: Type) (core_ord:core_data -> core_data -> Prop),
-    (core_data -> meminj -> semC Sems -> mem -> semC Semt -> mem -> Prop) ->
-    core_data -> meminj -> C0 -> mem -> Cn -> mem -> Prop.
+    list compiler_index -> meminj -> C0 -> mem -> Call -> mem -> Prop.
   Admitted. 
 
-  Notation Nconcur_match:=(All_concur_match' match_source match_target).
-  
+  Notation Nconcur_match:=(All_concur_match').
+
   Lemma All_compiled_thread_simulation:
-    exists (core_data: Type), exists (core_ord : core_data -> core_data -> Prop),
-      exists compiler_match, exists v:val,
+    exists v:val,
           HybridMachine_simulation
-            Sems Semt hb0 hball U genv ge_inv init_inv halt_inv
-            core_data core_ord 
-            (Nconcur_match core_data core_ord (match_states compiler_match))  v.  
+            Sems Semt hb0 hball U genv'
+            (list compiler_index) (list_order) 
+            (Nconcur_match)  v.  
   Proof.
   Admitted.
   
@@ -805,3 +694,4 @@ End AllThredCompiled.
 
 
 End HybridProofs.
+      
