concurrency/lifting.v
@@ -1,5 +1,8 @@
 From mathcomp.ssreflect Require Import ssreflect fintype.
 
+Require Import Omega.
+Require Import msl.Coqlib2.
+
 Require Import compcert.common.Memory.
 Require Import compcert.common.Globalenvs.
 
@@ -19,40 +22,49 @@ Require Import sepcomp.event_semantics.
 
 (** The X86 DryConc Machine*)
 Require Import concurrency.dry_context.
+Require Import concurrency.x86_context.
 
 (** The Clight DryConc Machine*)
-Require Import concurrency.DryMachineSource.
+Require Import concurrency.DryMachineSourceCore.
 
 (** The new machine simulation*)
 Require Import concurrency.machine_semantics. Import machine_semantics.
 Require Import concurrency.machine_simulation. Import Machine_sim.
 
-Module lifting (SEMT: Semantics) (Machine: MachinesSig with Module SEM := SEMT).
+(** The hybrid simulation proof*)
+Require Import concurrency.CoreSemantics_sum.
+Require Import concurrency.HybridMachine_simulation_proof.
+
+
+Set Bullet Behavior "Strict Subproofs".
+
+Module lifting.
   Section lifting.
-    Import THE_DRY_MACHINE_SOURCE.
-    Import THE_DRY_MACHINE_SOURCE.DMS.
-    Notation GS := (SEM.G).
-    Notation GT := (SEMT.G).
-    Variable gT : GT.
-    Variable gS : GS.
+    Import DMS.
+    Import X86Machines.
+    Notation GS := (DMS.SEM.G).
+    Notation GT := (SEM.G).
+    Definition gT : GT:= snd genv'.
+    Definition gS : GS:= fst genv'.
 
-    Notation semS := (SEM.Sem).
-    Notation semT := (SEMT.Sem).
+    Notation semS := (DMS.SEM.Sem).
+    Notation semT := (SEM.Sem).
 
-    Notation CT := (SEMT.C).
-    Notation CS := (SEM.C).
+    Notation CT := (SEM.C).
+    Notation CS := (DMS.SEM.C).
 
-    Definition ge_inv (geS : GS) (geT : GT) :=
-      genvs_domain_eq (Clight.genv_genv geS) (SEMT.getEnv geT).
+   (* I don't think we need these
+      Definition ge_inv (geS : GS) (geT : GT) :=
+      genvs_domain_eq (Clight.genv_genv geS) (SEM.getEnv geT). *)
 
-    Definition init_inv j (geS : GS) valsS mS (geT : GT) valsT mT :=
+   (* Definition init_inv j (geS : GS) valsS mS (geT : GT) valsT mT :=
       Mem.mem_inj j mS mT /\
       List.Forall2 (val_inject j) valsS valsT /\
-      Events.meminj_preserves_globals (Clight.genv_genv geS) j.
+      Events.meminj_preserves_globals (Clight.genv_genv geS) j. *)
 
-    Definition halt_inv j (geS : GS) rv1 mS (geT : GT) rv2 mT :=
+    (* Definition halt_inv j (geS : GS) rv1 mS (geT : GT) rv2 mT :=
       Mem.mem_inj j mS mT /\
-      val_inject j rv1 rv2.
+      val_inject j rv1 rv2. *)
 
     (* Lemma concur_whole_sim main psrc ptgt (sch : mySchedule.schedule) :
       Wholeprog_sim
@@ -64,50 +76,226 @@ Module lifting (SEMT: Semantics) (Machine: MachinesSig with Module SEM := SEMT).
       
     Admitted. *)
 
+    
+    
+    Context (p : Clight.program) (tp : Asm.program).
+    Hypothesis compiled : Compiler.simpl_transf_clight_program p = Errors.OK tp.
+
+    (** *First: lets realte the concurrent machines and Hybrid machines*)
+    Definition source_state_make_hybrid (st: DMS.FineConc.machine_state):
+          t HybridMachine.Resources (HybridMachine.Sem (Some 0) Sems Semt).
+          destruct st.
+          econstructor; eauto.
+          intros t; apply pool in t.
+          destruct t.
+          eapply Krun. simpl.
+          eapply SState.
+          simpl in c. exact c.
+          eapply Kblocked. simpl.
+          eapply SState.
+          simpl in c. exact c.
+          eapply Kresume; eauto. simpl.
+          eapply SState.
+          simpl in c. exact c.
+          eapply (Kinit v v0).
+    Defined.
+
+    Lemma source_step_to_hybrid:
+          forall sch psrc gS gT U st1 m1 st1' m1',
+          thread_step (new_DMachineSem sch psrc) gS U st1 m1 st1' m1' ->
+          thread_step (HybridMachine_simulation.HCSem (Sems) Semt (Some 0) sch)
+                      (gS, gT) U
+                      (source_state_make_hybrid st1) m1
+                      (source_state_make_hybrid st1') m1'.
+        Proof.
+          intros. inversion H; subst.
+          assert (Hcmpt_: HybridMachine.mem_compatible (Some 0) (Sems) Semt
+                                                       (source_state_make_hybrid st1) m1).
+          { inversion Hcmpt; destruct st1; constructor; eauto. }
+          assert (Htid_: containsThread_ (HybridMachine.ThreadPool (Some 0) (Sems) Semt)
+                                  (source_state_make_hybrid st1) tid) by
+              (destruct st1; apply Htid).
+          econstructor; eauto.
+          instantiate (1:= nil).
+          instantiate (1:= Hcmpt_).
+          instantiate (1:= Htid_).
+          inversion Htstep; subst.
+          econstructor; eauto.
+          - (*invariant*)
+            inversion Hinv; destruct st1; simpl in *; econstructor;eauto.
+            simpl. unfold containsThread; simpl.
+            unfold DMS.DryMachine.ThreadPool.containsThread in Htid; simpl.
+            + intros. destruct ( pool (Ordinal (n:=pos.n num_threads) (m:=i) cnti));
+                        inversion H0; subst. exists c0; auto.
+            + intros. clear - H1; simpl.
+              simpl in H1; eapply NPeano.Nat.ltb_lt in H1. omega.
+          - clear - Hcode.
+            simpl. instantiate (1 := SState _ _ c).
+            destruct st1; simpl in *.
+            clear - Hcode. simpl in Htid_.
+            replace Htid_ with Htid. Focus 2. apply proof_irr. 
+            rewrite Hcode; auto.
+          - simpl.
+            econstructor; eauto.
+            simpl. admit. (*What is this???*)
+
+          - simpl. unfold updThread; simpl; destruct st1; simpl.
+            f_equal. extensionality id.
+            replace Htid_ with Htid. Focus 2. apply proof_irr. 
+            if_tac; eauto.
+            replace Htid_ with Htid. Focus 2. apply proof_irr.
+            auto.
+        Admitted.
+
+        Lemma source_machine_step_to_hybrid:
+          forall sch psrc gS gT U U' tr tr' st1 m1 st1' m1',
+          machine_step (new_DMachineSem sch psrc) gS U tr st1 m1 U' tr' st1' m1' ->
+          machine_step (HybridMachine_simulation.HCSem (Sems) Semt (Some 0) sch)
+                      (gS, gT) U nil
+                      (source_state_make_hybrid st1) m1 U' nil
+                      (source_state_make_hybrid st1') m1'.
+         Proof.
+           intros. inversion H; subst.
+           - (*INIT thread*)
+             econstructor 1; eauto.
+             inversion Hcmpt; destruct st1; econstructor; eauto.
+             inversion Htstep; subst.
+             admit.
+           - econstructor 2; eauto.
+             inversion Hcmpt; destruct st1; econstructor; eauto.
+             inversion Htstep; subst.
+             admit.
+           - econstructor 3; eauto.
+             inversion Hcmpt; destruct st1; econstructor; eauto.
+             inversion Htstep; subst.
+             admit.
+           - econstructor 4; eauto.
+             admit.
+           - econstructor 5; eauto.
+             inversion Hcmpt; destruct st1'; econstructor; eauto.
+             inversion Hinv; destruct st1'; econstructor; eauto.
+             admit.
+             admit.
+             unfold HybridMachine.threadHalted.
+             inversion Hhalted; subst.
+             admit.
+           - econstructor 6; eauto.
+             intros HH; apply Htid.
+             destruct st1'; eauto.
+             admit.
+         Admitted.
+
+        Definition target_state_make_hybrid (st: FineConc.machine_state):
+          t HybridMachine.Resources (HybridMachine.Sem None (Sems) Semt).
+          destruct st.
+          econstructor; eauto.
+          intros t; apply pool in t.
+          destruct t.
+          eapply Krun. simpl.
+          eapply TState.
+          simpl in c. exact c.
+          eapply Kblocked. simpl.
+          eapply TState.
+          simpl in c. exact c.
+          eapply Kresume; eauto. simpl.
+          eapply TState.
+          simpl in c. exact c.
+          eapply (Kinit v v0).
+        Defined.
+
+        
+        Lemma target_hybrid_to_step:
+          forall sch ptgt gS gT U st2 m2 st2_ m2',
+          thread_step
+            (HybridMachine_simulation.HCSem (Sems) Semt None sch) 
+            (gS, gT) U (target_state_make_hybrid st2) m2 st2_ m2' ->
+          exists st2', st2_ = (target_state_make_hybrid st2') /\
+                  thread_step (DryConc.new_MachineSemantics sch ptgt) gT U st2 m2 st2' m2'.
+        Proof.
+        Admitted.
+        Lemma target_hybrid_to_plus:
+          forall sch ptgt gS gT U st2 m2 st2_ m2',
+          machine_semantics_lemmas.thread_step_plus
+            (HybridMachine_simulation.HCSem (Sems) Semt None sch) 
+            (gS, gT) U (target_state_make_hybrid st2) m2 st2_ m2' ->
+          exists st2', st2_ = (target_state_make_hybrid st2') /\
+                  machine_semantics_lemmas.thread_step_plus
+                    (DryConc.new_MachineSemantics sch ptgt) gT U st2 m2 st2' m2'.
+        Proof.
+        Admitted.
+        Lemma target_hybrid_to_star:
+          forall sch ptgt gS gT U st2 m2 st2_ m2',
+          machine_semantics_lemmas.thread_step_star
+            (HybridMachine_simulation.HCSem (Sems) Semt None sch) 
+            (gS, gT) U (target_state_make_hybrid st2) m2 st2_ m2' ->
+          exists st2', st2_ = (target_state_make_hybrid st2') /\
+                  machine_semantics_lemmas.thread_step_star
+                    (DryConc.new_MachineSemantics sch ptgt) gT U st2 m2 st2' m2'.
+        Proof.
+        Admitted.
+
+        Lemma target_hybrid_to_machine_step:
+          forall sch ptgt gS gT U U' tr tr' st2 m2 st2_ m2',
+            machine_step (HybridMachine_simulation.HCSem (Sems) Semt None sch) 
+                         (gS, gT) U tr' (target_state_make_hybrid st2) m2 U' tr st2_ m2' ->
+            exists st2', st2_ = (target_state_make_hybrid st2') /\
+                    machine_step (DryConc.new_MachineSemantics sch ptgt) gT U nil st2 m2 U' nil st2' m2'.
+          
+        Admitted.
+        
+
+    (** *Proof the simulation between the Clight_core and Asm machines*)
     Lemma concur_sim main psrc ptgt (sch : mySchedule.schedule) :
       Machine_sim
         (new_DMachineSem sch psrc)
-        (Machine.DryConc.new_MachineSemantics sch ptgt)
-        gS gT main
-        ge_inv init_inv halt_inv.
+        (DryConc.new_MachineSemantics sch ptgt)
+        (fst genv') (snd genv') main.
     Proof.
-      
-      (*Transitivity lemma*)
-      Lemma compose_machine_simulations:
-        forall G1 G2 G3 C1 C2 C3 TID SCH TR M, 
-        forall (Sem1: @ConcurSemantics G1 TID SCH TR C1 M)
-          (Sem2: @ConcurSemantics G2 TID SCH TR C2 M)
-          (Sem3: @ConcurSemantics G3 TID SCH TR C3 M)
-          g1 g2 g3 main ge_inv1 ge_inv2 init_inv1 init_inv2 halt_inv1 halt_inv2,
-        Machine_sim Sem1 Sem2 g1 g2 main ge_inv1 init_inv1 halt_inv1 ->
-        Machine_sim Sem2 Sem3 g2 g3 main ge_inv2 init_inv2 halt_inv2->
-        exists ge_inv3 init_inv3 halt_inv3,
-          (Machine_sim Sem1 Sem3 g1 g3 main ge_inv3 init_inv3 halt_inv3) .
-        
-      Admitted.
+      pose proof (All_compiled_thread_simulation p tp compiled sch).
+      simpl in H. 
+      destruct H as ( v & HH).
+      inversion HH.
+      eapply Build_Machine_sim with
+          (core_data:= list (compiler_index p tp compiled))
+          (core_ord:= (list_order p tp compiled))
+          (match_state:= fun cd mu c1 m1 c2 m2 =>
+           All_concur_match' p tp compiled sch
+                     cd mu (source_state_make_hybrid c1) m1 (target_state_make_hybrid c2) m2)
+      ; eauto.
+      - admit. (*initial*)
+      - clear - thread_diagram; intros.
+        destruct genv'.
+        eapply source_step_to_hybrid in H.
+        eapply thread_diagram in H0; eauto.
+        destruct genv'; eauto. 
+        destruct H0 as
+            (st2_ & m2' &  cd' & mu' & MATCH & STEPS).
+        destruct STEPS as [STEPS | [STEPS ORDER]].
+        + eapply target_hybrid_to_plus in STEPS.
+          destruct STEPS as (st2' & eqST2 & STEPS).
+          exists st2', m2', cd', mu'.
+          split; eauto. rewrite <- eqST2; eauto.
+        + eapply target_hybrid_to_star in STEPS.
+          destruct STEPS as (st2' & eqST2 & STEPS).
+          exists st2', m2', cd', mu'.
+          split; auto. rewrite <- eqST2; eauto.
+      - clear - machine_diagram; intros.
+        destruct genv'.
+        assert (HH: tr = nil /\ tr' = nil).
+        { inversion H; subst; auto. }
+        destruct HH as [HH1 HH2]. subst.
 
-      eapply compose_machine_simulations.
-      
-          
-      eapply Build_Machine_sim.
-      - admit. (*Order is well founded*) 
-      - admit. (*ge_in*)
-      - { admit. 
-         (* simpl;
-          unfold DryConc.init_machine', Machine.DryConc.init_machine';
-          intros.
-          destruct (DryMachine.init_mach psrc gS main vals1) eqn:HH;
-            inversion H.
-          subst t.
-          eexists; eexists.
-          unfold DryMachine.init_mach in HH.
-        rewrite /ge_inv /genvs_domain_eq; intros.
-        { repeat split; simpl; intros.
-          + destruct H as [id H].
-            exists id. *) }
-      - intros. 
+        eapply source_machine_step_to_hybrid in H.
+        eapply machine_diagram in H0; eauto.
+        destruct H0 as
+            (st2_ & m2' &  cd' & MATCH & STEPS).
+        eapply target_hybrid_to_machine_step in STEPS.
+        destruct STEPS as (st2' & eqST2' & STEPS).
+        exists st2', m2', cd', mu; split; auto.
+        rewrite <- eqST2'; auto.
+      - (*Running*) admit.
     Admitted.
-
+      
   End lifting.
 End lifting.
 
