concurrency/Asm_self_simulation.v
@@ -1,0 +1,8 @@
+Require Import compcert.ia32.Asm.
+
+Require Import concurrency.self_simulation.
+
+Definition Asm_self_simulation tp:
+    self_simulation (ia32.Asm.semantics tp) ia32.Asm.get_mem.
+Admitted.
+    
