concurrency/Clight_self_simulation.v
@@ -1,0 +1,8 @@
+Require Import Clight.
+
+Require Import concurrency.self_simulation.
+
+Definition Clight_self_simulation (p: program) :
+    self_simulation (Clight.semantics2 p) Clight.get_mem.
+Admitted.
+    
