concurrency/DryMachineSourceCore.v
@@ -1,0 +1,77 @@
+Require Import compcert.common.Memory.
+
+
+Require Import veric.compcert_rmaps.
+Require Import veric.juicy_mem.
+Require Import veric.res_predicates.
+
+(*IM using proof irrelevance!*)
+Require Import ProofIrrelevance.
+
+(* The concurrent machinery*)
+Require Import concurrency.scheduler.
+Require Import concurrency.TheSchedule.
+
+Require Import concurrency.concurrent_machine.
+Require Import concurrency.semantics.
+Require Import concurrency.juicy_machine. Import Concur.
+Require Import concurrency.dry_machine. Import Concur.
+(*Require Import concurrency.dry_machine_lemmas. *)
+Require Import concurrency.lksize.
+Require Import concurrency.permissions.
+
+Require Import concurrency.dry_context.
+Require Import concurrency.dry_machine_lemmas.
+Require Import concurrency.erased_machine.
+
+(*Semantics*)
+Require Import veric.Clight_core.
+Require Import veric.Clightcore_coop.
+Require Import sepcomp.event_semantics.
+Require Import veric.Clight_sim.
+Require Import concurrency.ClightCoreSemantincsForMachines.
+Require Import concurrency.Clight_bounds.
+
+(*SSReflect*)
+From mathcomp.ssreflect Require Import ssreflect ssrfun ssrbool ssrnat eqtype seq.
+Require Import Coq.ZArith.ZArith.
+Require Import PreOmega.
+Require Import concurrency.ssromega. (*omega in ssrnat *)
+Set Bullet Behavior "Strict Subproofs".
+
+Import Concur threadPool.
+
+  Module SCH:= THESCH.
+  Module SEM:= ClightCoreSEM.
+  (*Import SCH SEM.*)
+
+  (*Module DSEM := DryMachineShell SEM.
+  Module DryMachine <: ConcurrentMachine:= CoarseMachine SCH DSEM.
+  Notation DMachineSem:= DryMachine.MachineSemantics.
+  Notation new_DMachineSem:= DryMachine.new_MachineSemantics.
+  Notation dstate:= DryMachine.SIG.ThreadPool.t.
+  Notation dmachine_state:= DryMachine.MachState.
+  (*Module DTP:= DryMachine.SIG.ThreadPool.*)
+  Import DSEM.DryMachineLemmas event_semantics.*)
+
+  Module DMS  <: MachinesSig with Module SEM := ClightCoreSEM.
+     Module SEM:= ClightCoreSEM .
+
+     (*Old DSEM*)
+     Module DryMachine <: DryMachineSig SEM := DryMachineShell SEM.
+     Module ErasedMachine :=  ErasedMachineShell SEM.
+
+     Module DryConc <: ConcurrentMachine :=
+      CoarseMachine SCH DryMachine.
+     Notation DMachineSem:= DryConc.MachineSemantics.
+     Notation new_DMachineSem:= DryConc.new_MachineSemantics.
+
+     Module FineConc := concurrent_machine.FineMachine SCH DryMachine.
+     (** SC machine*)
+     Module SC := concurrent_machine.FineMachine SCH ErasedMachine.
+     Module DTP<: ThreadPoolSig:= DryConc.SIG.ThreadPool.
+
+     Import DryMachine DTP.
+
+  End DMS.
+  Module DryMachineLemmas := ThreadPoolWF SEM DMS.
