veric/Clightcore_coop.v
@@ -1,0 +1,80 @@
+Require Import sepcomp.semantics.
+Require Import sepcomp.semantics_lemmas.
+Require Import sepcomp.mem_lemmas.
+Require Import veric.base.
+Require Import veric.Clight_core.
+
+Lemma alloc_variables_mem_step: forall cenv vars m e e2 m'
+      (M: alloc_variables cenv e m vars e2 m'), mem_step m m'.
+Proof. intros.
+  induction M.
+  apply mem_step_refl.
+  eapply mem_step_trans.
+    eapply mem_step_alloc; eassumption. eassumption.
+Qed.
+
+Lemma bind_parameters_mem_step: forall cenv e m pars vargs m'
+      (M: bind_parameters cenv e m pars vargs m'), mem_step m m'.
+Proof. intros.
+  induction M.
+  apply mem_step_refl.
+  inv H0.
++ eapply mem_step_trans; try eassumption. simpl in H2.
+  eapply mem_step_store; eassumption.
++ eapply mem_step_trans; try eassumption.
+  eapply mem_step_storebytes; eassumption.
+Qed.
+
+Lemma CLC_corestep_mem:
+  forall (g : genv) (c : CC_core) (m : mem) (c' : CC_core) (m' : mem),
+    corestep cl_core_sem g c m c' m' -> mem_step m m'.
+Admitted.
+
+
+Program Definition CLC_memsem :
+  @MemSem Clight.genv (*(Genv.t fundef type)*) CC_core.
+apply Build_MemSem with (csem := cl_core_sem).
+exact CLC_corestep_mem.
+Defined.
+
+
+(*
+Lemma assign_loc_forward:
+      forall cenv t m b ofs v m'
+      (A: assign_loc cenv t m b ofs v m'),
+      mem_forward m m'.
+Proof.
+intros.
+induction A.
+ unfold Mem.storev in H0.
+ eapply store_forward; eassumption.
+ eapply storebytes_forward; eassumption.
+Qed.
+
+Lemma alloc_variables_forward: forall cenv vars m e e2 m'
+      (M: alloc_variables cenv e m vars e2 m'),
+      mem_forward m m'.
+Proof. intros.
+  induction M.
+  apply mem_forward_refl.
+  apply alloc_forward in H.
+  eapply mem_forward_trans; eassumption.
+Qed.
+
+Lemma cln_forward: forall (g : genv) (c : corestate)
+  (m : mem) (c' : corestate) (m' : mem),
+  corestep cl_core_sem g c m c' m' -> mem_forward m m'.
+Proof.
+intros.
+induction H; try apply mem_forward_refl; trivial.
+  eapply assign_loc_forward; eassumption.
+  eapply alloc_variables_forward; eassumption.
+  eapply freelist_forward; eassumption.
+Qed.
+Program Definition CLN_coop_sem :
+  CoopCoreSem Clight.genv (*(Genv.t fundef type)*) corestate.
+apply Build_CoopCoreSem with (coopsem := cl_core_sem).
+apply cln_forward.
+admit. (*This is the new readonly condition which should be easy to prove.*)
+Admitted.
+*)
